feat: prepare for RA consistency

eventstructure.v
@@ -1,5 +1,5 @@
 From Coq Require Import Relations Relation_Operators.
-From RelationAlgebra Require Import lattice rel kat_tac.
+From RelationAlgebra Require Import lattice monoid rel kat_tac rel.
 From mathcomp Require Import ssreflect ssrfun ssrbool ssrnat seq path.
 From mathcomp Require Import eqtype choice order finmap fintype.
 From event_struct Require Import utilities relations wftype ident.
@@ -38,6 +38,7 @@ From event_struct Require Import utilities relations wftype ident.
 
 Import Order.LTheory.
 Open Scope order_scope.
+Local Open Scope ra_terms.
 Import WfClosure.
 
 Set Implicit Arguments.
@@ -567,26 +568,70 @@ Qed.
 (*     Writes-Before relation                                                *)
 (* ************************************************************************* *)
 
-Definition sca_suffix : E -> seq E := suffix (fica_lt).
+Definition sca : hrel E E := (ca : hrel E E) ∩ (fun x y => x <> y).
 
-Definition contr_loc f : E -> seq E := 
-  fun e => (f ∘ (same_loc (lab e) \o lab)ᶠ) e.
+Definition rf_inv : hrel E E := fun x y => frf x = y.
 
-Definition contr_wrire f : E -> seq E := 
-  (is_write \o lab)ᶠ ∘ f ∘ (is_write \o lab)ᶠ.
+Definition wb1 : hrel E E := fun e1 e2 =>
+  (
+    ((same_loc (lab e1) (lab e2)) *
+    (is_write (lab e1))) * 
+    ((is_write (lab e2)) *
+    ((sca e1 e2)))
+  )%type.
 
-Definition frf_inv : E -> seq E := 
-  fun e => [seq x <- dom | frf x == e].
+Definition wb2 : hrel E E := fun e1 e2 =>
+  (
+    ((same_loc (lab e1) (lab e2)) *
+    (is_write (lab e1))) * 
+    ((is_write (lab e2)) *
+    (((hrel_dot _ _ _ sca rf_inv) e1 e2) * (e1 <> e2)))
+  )%type.
 
-(* wb := [W] ; (po ∪ rf)⁺ |loc ; [W] ∪ [W]; (po ∪ rf)⁺ ; rf⁻ ; [W] \ id *)
+(* wb := [W] ; (po ∪ rf)⁺ |loc ; [W] ∪ [W]; (po ∪ rf)⁺ |loc ; rf⁻ ; [W] \ id *)
 
-Definition fwb : {fsfun E -> seq E with [::]} := 
-  [fsfun x in (seq_fset tt dom) => 
-    (
-      contr_wrire (contr_loc sca_suffix) 
-      ∪
-      strictify (contr_wrire (frf_inv ∘ (contr_loc sca_suffix)))
-    ) x].
+Definition wb := wb1 ⊔ wb2.
+
+Definition rwb1 e1 e2 := 
+  (
+    ((same_loc (lab e1) (lab e2)) *
+    (is_read (lab e1))) * 
+    ((is_read (lab e2)) *
+    ((frf e1) <> (frf e2))) *
+    (sca (frf e1) e2)
+  )%type.
+
+Definition rwb2 e1 e2 := 
+  (
+    ((same_loc (lab e1) (lab e2)) *
+    (is_read (lab e1))) * 
+    ((is_read (lab e2)) *
+    ((wb1 ⋅ sca) (frf e1) e2))
+  )%type.
+
+Definition rwb : hrel E E := rwb1 ⊔ rwb2.
+
+Lemma wb_rbw : 
+  (exists x, wb^* x x) <->
+  exists x, rwb^* x x.
+Proof. Admitted.
+
+Definition frwb : {fsfun E -> seq E with [::]}. Admitted.
+
+Lemma frwbP e1 e2: 
+  reflect (rwb e1 e2) (e2 \in frwb e1).
+Proof. Admitted.
+
+Definition seq_contr (f : E -> seq E) (xs : seq E): {fsfun E -> seq E with [::]} :=
+  [fsfun x in seq_fset tt dom => [seq y <- f x | y \in xs]] .
+
+Export FinClosure.
+
+Definition fwb_cf (rs : seq E) := 
+  if rs is r :: _ then
+    (t_closure (seq_contr frwb rs) r r) ||
+    (~~ allrel (fun e1 e2 => ~~ e1 # e2) rs rs)
+  else false.
 
 
 End ExecEventStructure.
